Obviously needs a lot of cleanup, but we have a low-level spec on deep/shallow handlers now

coq-osiris/theories/program_logic/handler_rules.v
@@ -2,7 +2,7 @@ From iris.proofmode Require Import proofmode.
 
 From osiris Require Import base.
 From osiris.lang Require Import lang.
-From osiris.program_logic Require Import ewp tactics.
+From osiris.program_logic Require Import ewp tactics basic_rules.
 From osiris.semantics Require Import code.
 
 (* -------------------------------------------------------------------------- *)
@@ -15,6 +15,210 @@ Section handler_specifications.
   Context {A X : Type}.
 
 (* -------------------------------------------------------------------------- *)
+  (** * Deep handler specification. *)
+
+  Definition deep_handler_spec_pre
+    (deep_handler_spec:
+      coPset -d>
+      P -d>
+      (outcome2 val exn -d> iPropO Σ) -d>
+      (outcome3 val exn -> microvx) -d>
+      P -d>
+      (outcome2 val exn -d> iPropO Σ) -d>
+      iPropI Σ) :
+      coPset -d>
+      P -d>
+      (outcome2 val exn -d> iPropO Σ) -d>
+      (outcome3 val exn -> microvx) -d>
+      P -d>
+      (outcome2 val exn -d> iPropO Σ) -d>
+      iPropI Σ :=
+    (λ E Ψ Φ h Ψ' Φ',
+      ((* [Return] and [Exception] branch *)
+      (∀ o, Φ o -∗ ▷ EWP (h o) @ E <| Ψ' |> {{ Φ' }}) ∧
+
+      (* [Effect] branch *)
+      (∀ v k, Ψ allows perform v
+          << fun o : outcome2 val exn => ∀ Ψ'' Φ'',
+            ▷ deep_handler_spec E Ψ Φ h Ψ'' Φ'' -∗
+            EWP (stop CResume (k, o)) @ E <| Ψ'' |> {{ Φ'' }} >> -∗
+        ▷ EWP (h (O3Perform v k)) @ E <| Ψ' |> {{ Φ' }})))%I.
+
+  Local Instance deep_handler_spec_pre_contractive: Contractive deep_handler_spec_pre.
+  Proof.
+    rewrite /deep_handler_spec_pre /= => n wp wp' Hwp E m Φ.
+    repeat intro. repeat (f_contractive || f_equiv).
+    repeat intro. repeat (f_contractive || f_equiv).
+    apply Hwp.
+  Qed.
+
+  Local Definition deep_handler_spec_def := fixpoint deep_handler_spec_pre.
+
+  Local Definition deep_handler_spec_aux : seal (@deep_handler_spec_def).
+  Proof. by eexists. Qed.
+  Definition deep_handler_spec := deep_handler_spec_aux.(unseal).
+
+  Lemma deep_handler_spec_unfold {E} Ψ Φ Ψ' Φ' h :
+    deep_handler_spec E Ψ Φ h Ψ' Φ' ⊣⊢
+    deep_handler_spec_pre deep_handler_spec_def E Ψ Φ h Ψ' Φ'.
+  Proof.
+    rewrite /deep_handler_spec seal_eq /deep_handler_spec_def;
+    apply (@fixpoint_unfold _ _ _ deep_handler_spec_pre).
+  Qed.
+
+
+  (* TODO : Prove rule about [deep_handler_spec] (probably needs to be done at
+      the expr level). *)
+
+End handler_specifications.
+
+(* TODO : Move *)
+Definition outcome3_to_micro (o : outcome3 val exn) :=
+  match o with
+  | O3Ret a => Ret a
+  | O3Throw e => Throw e
+  | O3Perform e k => Stop CPerform e (fun v => stop CResume (k, v))
+  end.
+
+(* TODO : Move *)
+Notation "l ↦ v" := (gen_heap.mapsto l (DfracOwn 1) v)
+  (at level 20, format "l  ↦  v") : bi_scope.
+
+Opaque eval_match.
+
+Local Ltac ewp_invert :=
+  match goal with
+  | |- context [environments.Esnoc _ ?SI (state_interp _)] =>
+      match goal with
+      (* EWP throw *)
+      | |- context [environments.Esnoc _ ?Hwp (ewp_def _ (throw _) _ _)] =>
+          iPoseProof (ewp_throw_inv with "[$]") as "HΦ"
+      (* EWP ret *)
+      | |- context [environments.Esnoc _ ?Hwp (ewp_def _ (ret _) _ _)] =>
+          iMod (ewp_ret_inv with "[$]") as "HΦ"
+      (* EWP crash *)
+      | |- context [environments.Esnoc _ ?Hwp (ewp_def _ Crash _ _)] =>
+          match goal with
+          | |- context [environments.Esnoc _ ?SI (state_interp _)] =>
+            iMod (ewp_crash_inv with "[$][$]") as "%"
+          end
+      end
+  end.
+
+
+Section handler_proof.
+
+  Context `{!osirisGS Σ} `{protocol_wf Σ P}.
+
+  Context {A X : Type}.
+
+  Import ewp_rules_tactics.
+
+  Definition shallow_match η e bs :=
+    Handle (eval η e) (λ o, eval_shallow_match η o bs).
+
+  Definition deep_match η e bs :=
+    Handle (eval η e) (λ o, eval_deep_match η o bs).
+
+  Lemma ewp_shallow_match E Ψ Φ Ψ' Φ' η e bs:
+    EWP (eval η e) @ E <| Ψ |> {{ Φ }} -∗
+    (* The shallow handler specification is met *)
+    shallow_handler_spec E Ψ Φ (λ o, eval_shallow_match η o bs) Ψ' Φ' -∗
+    EWP (shallow_match η e bs) @ E <| Ψ' |> {{ Φ' }}.
+  Proof.
+    iIntros "He Hspec".
+    rewrite /shallow_match.
+    by iApply (ewp_handle with "He").
+  Qed.
+
+  Lemma ewp_deep_match E Ψ Φ Ψ' Φ' η e bs:
+    EWP (eval η e) @ E <| Ψ |> {{ Φ }} -∗
+    (* The deep handler specification is met *)
+    deep_handler_spec E Ψ Φ (λ o, pre_eval_match_aux eval true η o bs bs) Ψ' Φ' -∗
+    EWP (deep_match η e bs) @ E <| Ψ' |> {{ Φ' }}.
+  Proof.
+    (* We proceed by Löb-induction after generalizing [η] [e] and [bs]. *)
+    rewrite /deep_match. remember (eval η e). clear.
+    iLöb as "IH" forall (m η bs Ψ' Φ').
+
+    iIntros "He Hsh".
+    ewp_unfold_head.
+    intro_state.
+
+    ewp_mask_intro "Hmod".
+    Opaque eval_deep_match.
+    construct_wp_nonret; destruct_step; cbn; iMod "Hmod" as "_"; try rewrite -x; cbn;
+    rewrite !deep_handler_spec_unfold /deep_handler_spec_pre /=.
+
+    1,2: (* [StepHandleRet] and [StepHandleThrow] *)
+      ewp_invert; iFrame;
+      iDestruct "Hsh" as "[Hsh _]";
+      iSpecialize ("Hsh" with "HΦ");
+      try iMod "Hsh";
+      by ewp_mask_intro "Hmod"; ewp_mask_elim.
+
+    { (* [StepHandlePerform] *)
+      iDestruct "Hsh" as "[_ Hsh]".
+      iPoseProof (ewp_perform_inv with "[$]") as "HP".
+      iMod "HP".
+
+      iDestruct (gen_heap.gen_heap_alloc _ _ (K k) with "Hsi") as ">[Hsi [HH _]]";
+        [ exact H0 | ].
+      iFrame.
+
+      Transparent eval_deep_match.
+      rewrite {2}/eval_deep_match.
+      Opaque eval_deep_match.
+      cbn.
+
+      iApply (ewp_install with "HH").
+      ewp_mask_intro "Hmod"; ewp_mask_elim.
+      iIntros (?) "Hl"; cbn.
+
+      iAssert (Ψ allows perform e
+        << λ o : outcome2 val exn,
+            ∀ Ψ'' Φ'',
+              ▷ deep_handler_spec_def E Ψ Φ (λ o, pre_eval_match_aux eval true η o bs bs) Ψ'' Φ'' -∗
+              EWP stop CResume (l', o) @ E <| Ψ'' |> {{ Φ'' }} >>)%I
+        with "[HP Hl]" as "HΨ".
+      { iApply prot_mono_post; iFrame.
+        iIntros (?) "Hwp"; cbn.
+        iIntros (??) "H".
+        iSpecialize ("IH" with "Hwp").
+
+        rewrite /deep_handler_spec seal_eq.
+
+        iApply (ewp_resume with "Hl"). iNext.
+        iIntros (?) "Hl". cbn.
+        iSpecialize ("IH" with "H").
+
+        erewrite (eq_handle_handle (k w) (λ o : outcome3 C.val C.exn, try2 (eval_match η o bs) inject2)).
+        2 : intros; rewrite try2_ret_right; reflexivity.
+        done. } (* We're forgetting the [Shot] information here *)
+
+      iSpecialize ("Hsh" with "HΨ"). Transparent eval_deep_match.
+      rewrite /eval_deep_match /pre_eval_match. done. }
+
+    { (* [StepHandleCrash] *)
+      by ewp_invert. }
+
+    { (* [StepHandleLeft] *)
+      iPoseProof (ewp_step _ _ _ _ Hstep with "Hsi He") as ">H".
+      ewp_mask_elim. iMod "H" as "[$ H]". iModIntro.
+      iSpecialize ("IH" with "H").
+      rewrite deep_handler_spec_unfold.
+      iApply ("IH" with "Hsh"). }
+  Qed.
+
+End handler_proof.
+
+Section alternative_handler_specifications.
+
+  Context `{!osirisGS Σ} `{protocol_wf Σ P}.
+
+  Context {A X : Type}.
+
+ (* -------------------------------------------------------------------------- *)
   (** * Shallow handler specification. *)
 
   Definition shallow_handler_spec_pre
@@ -41,7 +245,7 @@ Section handler_specifications.
       (∀ (o : outcome2 val exn) e,
         Φ o -∗
         ⌜try_cextend_pure η o bs = Some e⌝ -∗
-        ▷ EWP e @ E <| Ψ' |> {{ Φ' }}) ∧
+        EWP e @ E <| Ψ' |> {{ Φ' }}) ∧
 
      (* Effectful branch. *)
       (∀ v k η' e,
@@ -73,61 +277,6 @@ Section handler_specifications.
   Proof. by eexists. Qed.
   Definition shallow_handler_spec := shallow_handler_spec_aux.(unseal).
 
-(* -------------------------------------------------------------------------- *)
-  (** * Deep handler specification. *)
-
-  Definition deep_handler_spec_pre
-    (deep_handler_spec:
-      coPset -d>
-      P -d>
-      (outcome2 val exn -d> iPropO Σ) -d>
-      (outcome3 val exn -> microvx) -d>
-      P -d>
-      (outcome2 val exn -d> iPropO Σ) -d>
-      iPropI Σ) :
-      coPset -d>
-      P -d>
-      (outcome2 val exn -d> iPropO Σ) -d>
-      (outcome3 val exn -> microvx) -d>
-      P -d>
-      (outcome2 val exn -d> iPropO Σ) -d>
-      iPropI Σ :=
-    (λ E Ψ Φ h Ψ' Φ',
-      ((* [Return] and [Exception] branch *)
-      (∀ o, Φ o -∗ ▷ EWP (h o) @ E <| Ψ' |> {{ Φ' }}) ∧
-
-      (* [Effect] branch *)
-      (∀ v k, Ψ allows perform v
-          << fun o => ∀ Ψ'' Φ'',
-            ▷ deep_handler_spec E Ψ Φ h Ψ'' Φ'' -∗
-            EWP (stop CResume (k, o)) @ E <| Ψ'' |> {{ Φ'' }} >> -∗
-        ▷ EWP (h (O3Perform v k)) @ E <| Ψ' |> {{ Φ' }})))%I.
-
-  Local Instance deep_handler_spec_pre_contractive: Contractive deep_handler_spec_pre.
-  Proof.
-    rewrite /deep_handler_spec_pre /= => n wp wp' Hwp E m Φ.
-    repeat intro. repeat (f_contractive || f_equiv).
-    repeat intro. repeat (f_contractive || f_equiv).
-    apply Hwp.
-  Qed.
-
-  Definition deep_handler_spec_def := fixpoint deep_handler_spec_pre.
-
-  Local Definition deep_handler_spec_aux : seal (@deep_handler_spec_def).
-  Proof. by eexists. Qed.
-  Definition deep_handler_spec := deep_handler_spec_aux.(unseal).
-
-  (* TODO : Prove rule about [deep_handler_spec] (probably needs to be done at
-      the expr level). *)
-
-End handler_specifications.
-
-Section handler_proof.
-
-  Context `{!osirisGS Σ} `{protocol_wf Σ P}.
-
-  Context {A X : Type}.
-
   Lemma shallow_handler_spec_unfold {E} Ψ Φ Ψ' Φ' η bs :
     shallow_handler_spec E Ψ Φ Ψ' Φ' η bs ⊣⊢
     shallow_handler_spec_pre shallow_handler_spec_def E Ψ Φ Ψ' Φ' η bs.
@@ -136,23 +285,11 @@ Section handler_proof.
     apply (@fixpoint_unfold _ _ _ shallow_handler_spec_pre).
   Qed.
 
-  Local Ltac spec_unfold :=
-    rewrite !shallow_handler_spec_unfold /shallow_handler_spec_pre /=.
+End alternative_handler_specifications.
 
-  Lemma ewp_shallow_handler E Ψ Φ Ψ' Φ' η o bs:
-    ⌜try_cextend_pure η o bs = None⌝ -∗
-    shallow_handler_spec E Ψ Φ Ψ' Φ' η bs -∗
-    EWP (eval_shallow_match η o bs) @ E <| Ψ' |> {{ Φ' }}.
-  Proof.
-    (* Induction on the handler, which is a list of branches *)
-    iInduction bs as [ | ] "IH".
-    { (* Empty handler. *)
-      iIntros "Hspec"; spec_unfold.
-      cbn; destruct o.
 
-      (* [O3Ret] case *)
-      -
+(* ------------------------------------------------------------------------ *)
+  (* Local tactics *)
 
-  Admitted.
-  
-End handler_proof.
+Local Ltac spec_unfold :=
+  rewrite !shallow_handler_spec_unfold /shallow_handler_spec_pre /=.
